column round boilerplate

examples/riscv/chacha/chacha_column_round_propScript.sml
@@ -38,6 +38,56 @@ open chacha_symb_transf_column_roundTheory;
 
 val _ = new_theory "chacha_column_round_prop";
 
+Definition riscv_chacha_quarter_round_exprs_def:
+ riscv_chacha_quarter_round_exprs pre_a pre_b pre_c pre_d
+  : word32 # word32 # word32 # word32 =
+  let a = pre_a in
+  let b = pre_b in
+  let c = pre_c in
+  let d = pre_d in
+
+  let a = riscv_chacha_line_exp_fst a b in
+  let d = riscv_chacha_line_exp_snd a d 16w in
+
+  let c = riscv_chacha_line_exp_fst c d in
+  let b = riscv_chacha_line_exp_snd c b 12w in
+
+  let a = riscv_chacha_line_exp_fst a b in
+  let d = riscv_chacha_line_exp_snd a d 8w in
+
+  let c = riscv_chacha_line_exp_fst c d in
+  let b = riscv_chacha_line_exp_snd c b 7w in
+
+  (a,b,c,d)
+End
+
+Definition riscv_chacha_column_round_exprs_def:
+ riscv_chacha_column_round_exprs 
+  pre_arr_0 pre_arr_1 pre_arr_2 pre_arr_3
+  pre_arr_4 pre_arr_5 pre_arr_6 pre_arr_7
+  pre_arr_8 pre_arr_9 pre_arr_10 pre_arr_11
+  pre_arr_12 pre_arr_13 pre_arr_14 pre_arr_15
+ : word32 # word32 # word32 # word32 #
+   word32 # word32 # word32 # word32 #
+   word32 # word32 # word32 # word32 #
+   word32 # word32 # word32 # word32
+  =
+ let (arr_0,arr_4,arr_8,arr_12) =
+   riscv_chacha_quarter_round_exprs pre_arr_0 pre_arr_4 pre_arr_8 pre_arr_12
+ in
+ let (arr_1,arr_5,arr_9,arr_13) =
+   riscv_chacha_quarter_round_exprs pre_arr_1 pre_arr_5 pre_arr_9 pre_arr_13
+ in
+ let (arr_2,arr_6,arr_10,arr_14) =
+   riscv_chacha_quarter_round_exprs pre_arr_2 pre_arr_6 pre_arr_10 pre_arr_14
+ in
+ let (arr_3,arr_7,arr_11,arr_15) =
+   riscv_chacha_quarter_round_exprs pre_arr_3 pre_arr_7 pre_arr_11 pre_arr_15
+ in
+ (arr_0,arr_1,arr_2,arr_3,arr_4,arr_5,arr_6,arr_7,
+  arr_8,arr_9,arr_10,arr_11,arr_12,arr_13,arr_14,arr_15)
+End
+
 Definition riscv_chacha_column_round_pre_def:
  riscv_chacha_column_round_pre 
   (pre_arr_0:word32) (pre_arr_1:word32) (pre_arr_2:word32) (pre_arr_3:word32)
@@ -45,7 +95,22 @@ Definition riscv_chacha_column_round_pre_def:
   (pre_arr_8:word32) (pre_arr_9:word32) (pre_arr_10:word32) (pre_arr_11:word32) 
   (pre_arr_12:word32) (pre_arr_13:word32) (pre_arr_14:word32) (pre_arr_15:word32)
  (m:riscv_state) : bool =
- (T)
+ (n2w (w2n (m.c_gpr m.procID 10w)) = pre_arr_0 /\
+  n2w (w2n (m.c_gpr m.procID 16w)) = pre_arr_1 /\
+  n2w (w2n (m.c_gpr m.procID 17w)) = pre_arr_2 /\
+  n2w (w2n (m.c_gpr m.procID 6w)) = pre_arr_3 /\
+  n2w (w2n (m.c_gpr m.procID 22w)) = pre_arr_4 /\
+  n2w (w2n (m.c_gpr m.procID 11w)) = pre_arr_5 /\
+  n2w (w2n (m.c_gpr m.procID 13w)) = pre_arr_6 /\
+  n2w (w2n (m.c_gpr m.procID 14w)) = pre_arr_7 /\
+  n2w (w2n (m.c_gpr m.procID 28w)) = pre_arr_8 /\
+  n2w (w2n (m.c_gpr m.procID 29w)) = pre_arr_9 /\
+  n2w (w2n (m.c_gpr m.procID 30w)) = pre_arr_10 /\
+  n2w (w2n (m.c_gpr m.procID 31w)) = pre_arr_11 /\
+  n2w (w2n (m.c_gpr m.procID 26w)) = pre_arr_12 /\
+  n2w (w2n (m.c_gpr m.procID 25w)) = pre_arr_13 /\
+  n2w (w2n (m.c_gpr m.procID 24w)) = pre_arr_14 /\
+  n2w (w2n (m.c_gpr m.procID 23w)) = pre_arr_15)
 End
 
 Definition riscv_chacha_column_round_post_def:
@@ -55,7 +120,28 @@ Definition riscv_chacha_column_round_post_def:
   (pre_arr_8:word32) (pre_arr_9:word32) (pre_arr_10:word32) (pre_arr_11:word32) 
   (pre_arr_12:word32) (pre_arr_13:word32) (pre_arr_14:word32) (pre_arr_15:word32)
  (m:riscv_state) : bool =
- (T)
+ (let (arr_0,arr_1,arr_2,arr_3,arr_4,arr_5,arr_6,arr_7,arr_8,
+       arr_9,arr_10,arr_11,arr_12,arr_13,arr_14,arr_15) =
+   riscv_chacha_column_round_exprs
+     pre_arr_0 pre_arr_1 pre_arr_2 pre_arr_3 pre_arr_4 pre_arr_5 pre_arr_6 pre_arr_7
+     pre_arr_8 pre_arr_9 pre_arr_10 pre_arr_11 pre_arr_12 pre_arr_13 pre_arr_14 pre_arr_15
+  in
+  n2w (w2n (m.c_gpr m.procID 20w)) = arr_0 /\
+  n2w (w2n (m.c_gpr m.procID 19w)) = arr_1 /\
+  n2w (w2n (m.c_gpr m.procID 18w)) = arr_2 /\
+  n2w (w2n (m.c_gpr m.procID 9w)) = arr_3 /\
+  n2w (w2n (m.c_gpr m.procID 21w)) = arr_4 /\
+  n2w (w2n (m.c_gpr m.procID 10w)) = arr_5 /\
+  n2w (w2n (m.c_gpr m.procID 13w)) = arr_6 /\
+  n2w (w2n (m.c_gpr m.procID 14w)) = arr_7 /\
+  n2w (w2n (m.c_gpr m.procID 8w)) = arr_8 /\
+  n2w (w2n (m.c_gpr m.procID 7w)) = arr_9 /\
+  n2w (w2n (m.c_gpr m.procID 5w)) = arr_10 /\
+  n2w (w2n (m.c_gpr m.procID 15w)) = arr_11 /\
+  n2w (w2n (m.c_gpr m.procID 22w)) = arr_12 /\
+  n2w (w2n (m.c_gpr m.procID 28w)) = arr_13 /\
+  n2w (w2n (m.c_gpr m.procID 29w)) = arr_14 /\
+  n2w (w2n (m.c_gpr m.procID 16w)) = arr_15)
 End
 
 (* ------------------------------------- *)
@@ -65,13 +151,20 @@ End
 Theorem chacha_column_round_riscv_pre_imp_bspec_pre_thm:
  bir_pre_riscv_to_bir
   (riscv_chacha_column_round_pre pre_arr_0 pre_arr_1 pre_arr_2 pre_arr_3 pre_arr_4 pre_arr_5 pre_arr_6
-    pre_arr_7 pre_arr_8 pre_arr_9 pre_arr_10 pre_arr_11 pre_arr_12
-    pre_arr_13 pre_arr_14 pre_arr_15)
+    pre_arr_7 pre_arr_8 pre_arr_9 pre_arr_10 pre_arr_11 pre_arr_12 pre_arr_13 pre_arr_14 pre_arr_15)
   (bspec_chacha_column_round_pre pre_arr_0 pre_arr_1 pre_arr_2 pre_arr_3 pre_arr_4 pre_arr_5 pre_arr_6
-    pre_arr_7 pre_arr_8 pre_arr_9 pre_arr_10 pre_arr_11 pre_arr_12
-    pre_arr_13 pre_arr_14 pre_arr_15)
+    pre_arr_7 pre_arr_8 pre_arr_9 pre_arr_10 pre_arr_11 pre_arr_12 pre_arr_13 pre_arr_14 pre_arr_15)
 Proof 
- cheat
+ rw [bir_pre_riscv_to_bir_def,riscv_chacha_column_round_pre_def,bspec_chacha_column_round_pre_def] >-
+  (rw [bir_is_bool_exp_REWRS,bir_is_bool_exp_env_REWRS] >>
+   FULL_SIMP_TAC (std_ss++holBACore_ss) [bir_typing_expTheory.type_of_bir_exp_def]) >>
+ FULL_SIMP_TAC (std_ss++holBACore_ss) [
+  riscv_bmr_rel_EVAL,bir_val_TF_bool2b_DEF,
+  bool2b_def,
+  bool2w_def,
+  w2w_n2w_w2n_64_32
+ ] >>
+ EVAL_TAC
 QED
 
 Theorem chacha_column_round_riscv_post_imp_bspec_post_thm:
